formal/fstar/ocaml-output/RML_Mapping.ml
@@ -1,0 +1,730 @@
+open Prims
+let rml_TriplesMap : RDF_Graph_Executable.wf_iri=
+  "http://w3id.org/rml/TriplesMap"
+let rml_baseIRI : RDF_Graph_Executable.wf_iri= "http://w3id.org/rml/baseIRI"
+let rml_logicalSource : RDF_Graph_Executable.wf_iri=
+  "http://w3id.org/rml/logicalSource"
+let rml_iterator : RDF_Graph_Executable.wf_iri=
+  "http://w3id.org/rml/iterator"
+let rml_referenceFormulation : RDF_Graph_Executable.wf_iri=
+  "http://w3id.org/rml/referenceFormulation"
+let rml_JSONPath : RDF_Graph_Executable.wf_iri=
+  "http://w3id.org/rml/JSONPath"
+let rml_XPath : RDF_Graph_Executable.wf_iri= "http://w3id.org/rml/XPath"
+let rml_CSV : RDF_Graph_Executable.wf_iri= "http://w3id.org/rml/CSV"
+let rml_source : RDF_Graph_Executable.wf_iri= "http://w3id.org/rml/source"
+let rml_path : RDF_Graph_Executable.wf_iri= "http://w3id.org/rml/path"
+let rml_root : RDF_Graph_Executable.wf_iri= "http://w3id.org/rml/root"
+let rml_null : RDF_Graph_Executable.wf_iri= "http://w3id.org/rml/null"
+let rml_MappingDirectory : RDF_Graph_Executable.wf_iri=
+  "http://w3id.org/rml/MappingDirectory"
+let rml_CurrentWorkingDirectory : RDF_Graph_Executable.wf_iri=
+  "http://w3id.org/rml/CurrentWorkingDirectory"
+let rml_subjectMap : RDF_Graph_Executable.wf_iri=
+  "http://w3id.org/rml/subjectMap"
+let rml_subject : RDF_Graph_Executable.wf_iri= "http://w3id.org/rml/subject"
+let rml_class : RDF_Graph_Executable.wf_iri= "http://w3id.org/rml/class"
+let rml_graph : RDF_Graph_Executable.wf_iri= "http://w3id.org/rml/graph"
+let rml_graphMap : RDF_Graph_Executable.wf_iri=
+  "http://w3id.org/rml/graphMap"
+let rml_defaultGraph : RDF_Graph_Executable.wf_iri=
+  "http://w3id.org/rml/defaultGraph"
+let rml_predicateObjectMap : RDF_Graph_Executable.wf_iri=
+  "http://w3id.org/rml/predicateObjectMap"
+let rml_predicate : RDF_Graph_Executable.wf_iri=
+  "http://w3id.org/rml/predicate"
+let rml_predicateMap : RDF_Graph_Executable.wf_iri=
+  "http://w3id.org/rml/predicateMap"
+let rml_object : RDF_Graph_Executable.wf_iri= "http://w3id.org/rml/object"
+let rml_objectMap : RDF_Graph_Executable.wf_iri=
+  "http://w3id.org/rml/objectMap"
+let rml_parentTriplesMap : RDF_Graph_Executable.wf_iri=
+  "http://w3id.org/rml/parentTriplesMap"
+let rml_joinCondition : RDF_Graph_Executable.wf_iri=
+  "http://w3id.org/rml/joinCondition"
+let rml_child : RDF_Graph_Executable.wf_iri= "http://w3id.org/rml/child"
+let rml_parent : RDF_Graph_Executable.wf_iri= "http://w3id.org/rml/parent"
+let rml_childMap : RDF_Graph_Executable.wf_iri=
+  "http://w3id.org/rml/childMap"
+let rml_parentMap : RDF_Graph_Executable.wf_iri=
+  "http://w3id.org/rml/parentMap"
+let rml_constant : RDF_Graph_Executable.wf_iri=
+  "http://w3id.org/rml/constant"
+let rml_reference : RDF_Graph_Executable.wf_iri=
+  "http://w3id.org/rml/reference"
+let rml_template : RDF_Graph_Executable.wf_iri=
+  "http://w3id.org/rml/template"
+let rml_termType : RDF_Graph_Executable.wf_iri=
+  "http://w3id.org/rml/termType"
+let rml_IRI : RDF_Graph_Executable.wf_iri= "http://w3id.org/rml/IRI"
+let rml_URI : RDF_Graph_Executable.wf_iri= "http://w3id.org/rml/URI"
+let rml_UnsafeIRI : RDF_Graph_Executable.wf_iri=
+  "http://w3id.org/rml/UnsafeIRI"
+let rml_BlankNode : RDF_Graph_Executable.wf_iri=
+  "http://w3id.org/rml/BlankNode"
+let rml_Literal : RDF_Graph_Executable.wf_iri= "http://w3id.org/rml/Literal"
+let rml_datatype : RDF_Graph_Executable.wf_iri=
+  "http://w3id.org/rml/datatype"
+let rml_datatypeMap : RDF_Graph_Executable.wf_iri=
+  "http://w3id.org/rml/datatypeMap"
+let rml_language : RDF_Graph_Executable.wf_iri=
+  "http://w3id.org/rml/language"
+let rml_languageMap : RDF_Graph_Executable.wf_iri=
+  "http://w3id.org/rml/languageMap"
+type template_segment =
+  | TSeg_Literal of Prims.string 
+  | TSeg_Reference of Prims.string 
+let uu___is_TSeg_Literal (projectee : template_segment) : Prims.bool=
+  match projectee with | TSeg_Literal _0 -> true | uu___ -> false
+let __proj__TSeg_Literal__item___0 (projectee : template_segment) :
+  Prims.string= match projectee with | TSeg_Literal _0 -> _0
+let uu___is_TSeg_Reference (projectee : template_segment) : Prims.bool=
+  match projectee with | TSeg_Reference _0 -> true | uu___ -> false
+let __proj__TSeg_Reference__item___0 (projectee : template_segment) :
+  Prims.string= match projectee with | TSeg_Reference _0 -> _0
+let flush_template_buf (mode : Prims.bool) (buf : Prims.string)
+  (acc : template_segment Prims.list) : template_segment Prims.list=
+  if buf = ""
+  then acc
+  else
+    if mode then (TSeg_Reference buf) :: acc else (TSeg_Literal buf) :: acc
+let rec scan_template_acc (s : Prims.string) (pos : Prims.nat)
+  (fuel : Prims.nat) (mode : Prims.bool) (buf : Prims.string)
+  (acc : template_segment Prims.list) : template_segment Prims.list=
+  if fuel = Prims.int_zero
+  then flush_template_buf mode buf acc
+  else
+    (let len = FStar_String.strlen s in
+     if pos >= len
+     then flush_template_buf mode buf acc
+     else
+       (let c = FStar_Char.int_of_char (FStar_String.index s pos) in
+        if (c = (Prims.of_int (0x5C))) && ((pos + Prims.int_one) < len)
+        then
+          scan_template_acc s (pos + (Prims.of_int (2)))
+            (fuel - Prims.int_one) mode
+            (Prims.strcat buf
+               (FStar_String.sub s (pos + Prims.int_one) Prims.int_one)) acc
+        else
+          if (Prims.op_Negation mode) && (c = (Prims.of_int (0x7B)))
+          then
+            (let acc' = if buf = "" then acc else (TSeg_Literal buf) :: acc in
+             scan_template_acc s (pos + Prims.int_one) (fuel - Prims.int_one)
+               true "" acc')
+          else
+            if mode && (c = (Prims.of_int (0x7D)))
+            then
+              scan_template_acc s (pos + Prims.int_one)
+                (fuel - Prims.int_one) false "" ((TSeg_Reference buf) :: acc)
+            else
+              scan_template_acc s (pos + Prims.int_one)
+                (fuel - Prims.int_one) mode
+                (Prims.strcat buf (FStar_String.sub s pos Prims.int_one)) acc))
+let parse_template (s : Prims.string) : template_segment Prims.list=
+  FStar_List_Tot_Base.rev
+    (scan_template_acc s Prims.int_zero
+       ((FStar_String.strlen s) + Prims.int_one) false "" [])
+type term_type =
+  | TT_IRI 
+  | TT_URI 
+  | TT_UnsafeIRI 
+  | TT_BlankNode 
+  | TT_Literal 
+let uu___is_TT_IRI (projectee : term_type) : Prims.bool=
+  match projectee with | TT_IRI -> true | uu___ -> false
+let uu___is_TT_URI (projectee : term_type) : Prims.bool=
+  match projectee with | TT_URI -> true | uu___ -> false
+let uu___is_TT_UnsafeIRI (projectee : term_type) : Prims.bool=
+  match projectee with | TT_UnsafeIRI -> true | uu___ -> false
+let uu___is_TT_BlankNode (projectee : term_type) : Prims.bool=
+  match projectee with | TT_BlankNode -> true | uu___ -> false
+let uu___is_TT_Literal (projectee : term_type) : Prims.bool=
+  match projectee with | TT_Literal -> true | uu___ -> false
+type reference_formulation =
+  | RF_JSONPath 
+  | RF_XPath 
+  | RF_CSV 
+  | RF_Other of Prims.string 
+let uu___is_RF_JSONPath (projectee : reference_formulation) : Prims.bool=
+  match projectee with | RF_JSONPath -> true | uu___ -> false
+let uu___is_RF_XPath (projectee : reference_formulation) : Prims.bool=
+  match projectee with | RF_XPath -> true | uu___ -> false
+let uu___is_RF_CSV (projectee : reference_formulation) : Prims.bool=
+  match projectee with | RF_CSV -> true | uu___ -> false
+let uu___is_RF_Other (projectee : reference_formulation) : Prims.bool=
+  match projectee with | RF_Other _0 -> true | uu___ -> false
+let __proj__RF_Other__item___0 (projectee : reference_formulation) :
+  Prims.string= match projectee with | RF_Other _0 -> _0
+type source_root =
+  | Root_MappingDirectory 
+  | Root_CurrentWorkingDirectory 
+  | Root_Other of Prims.string 
+let uu___is_Root_MappingDirectory (projectee : source_root) : Prims.bool=
+  match projectee with | Root_MappingDirectory -> true | uu___ -> false
+let uu___is_Root_CurrentWorkingDirectory (projectee : source_root) :
+  Prims.bool=
+  match projectee with
+  | Root_CurrentWorkingDirectory -> true
+  | uu___ -> false
+let uu___is_Root_Other (projectee : source_root) : Prims.bool=
+  match projectee with | Root_Other _0 -> true | uu___ -> false
+let __proj__Root_Other__item___0 (projectee : source_root) : Prims.string=
+  match projectee with | Root_Other _0 -> _0
+let decode_term_type (t : RDF_Graph_Executable.rdf_term) :
+  term_type FStar_Pervasives_Native.option=
+  match t with
+  | RDF_Graph_Executable.T_IRI i ->
+      if i = rml_IRI
+      then FStar_Pervasives_Native.Some TT_IRI
+      else
+        if i = rml_URI
+        then FStar_Pervasives_Native.Some TT_URI
+        else
+          if i = rml_UnsafeIRI
+          then FStar_Pervasives_Native.Some TT_UnsafeIRI
+          else
+            if i = rml_BlankNode
+            then FStar_Pervasives_Native.Some TT_BlankNode
+            else
+              if i = rml_Literal
+              then FStar_Pervasives_Native.Some TT_Literal
+              else FStar_Pervasives_Native.None
+  | uu___ -> FStar_Pervasives_Native.None
+let decode_reference_formulation (t : RDF_Graph_Executable.rdf_term) :
+  reference_formulation=
+  match t with
+  | RDF_Graph_Executable.T_IRI i ->
+      if i = rml_JSONPath
+      then RF_JSONPath
+      else
+        if i = rml_XPath
+        then RF_XPath
+        else if i = rml_CSV then RF_CSV else RF_Other i
+  | uu___ -> RF_Other ""
+let decode_source_root (t : RDF_Graph_Executable.rdf_term) : source_root=
+  match t with
+  | RDF_Graph_Executable.T_IRI i ->
+      if i = rml_MappingDirectory
+      then Root_MappingDirectory
+      else
+        if i = rml_CurrentWorkingDirectory
+        then Root_CurrentWorkingDirectory
+        else Root_Other i
+  | uu___ -> Root_Other ""
+type node_ref = Prims.string
+let term_to_node_ref (t : RDF_Graph_Executable.rdf_term) :
+  node_ref FStar_Pervasives_Native.option=
+  match t with
+  | RDF_Graph_Executable.T_IRI i -> FStar_Pervasives_Native.Some i
+  | RDF_Graph_Executable.T_BNode b ->
+      FStar_Pervasives_Native.Some (Prims.strcat "_:" b)
+  | RDF_Graph_Executable.T_Literal uu___ -> FStar_Pervasives_Native.None
+let subject_to_node_ref (s : RDF_Graph_Executable.subject) : node_ref=
+  match s with
+  | RDF_Graph_Executable.S_IRI i -> i
+  | RDF_Graph_Executable.S_BNode b -> Prims.strcat "_:" b
+let rec distinct_subjects_acc (g : RDF_Graph_Executable.rdf_graph)
+  (acc : RDF_Graph_Executable.subject Prims.list) :
+  RDF_Graph_Executable.subject Prims.list=
+  match g with
+  | [] -> acc
+  | t::rest ->
+      if
+        FStar_List_Tot_Base.existsb
+          (RDF_Graph_Executable.subject_eq t.RDF_Graph_Executable.s) acc
+      then distinct_subjects_acc rest acc
+      else distinct_subjects_acc rest ((t.RDF_Graph_Executable.s) :: acc)
+let distinct_subjects (g : RDF_Graph_Executable.rdf_graph) :
+  RDF_Graph_Executable.subject Prims.list= distinct_subjects_acc g []
+type logical_source =
+  {
+  ls_iterator: Prims.string FStar_Pervasives_Native.option ;
+  ls_reference_formulation:
+    reference_formulation FStar_Pervasives_Native.option ;
+  ls_source_path: Prims.string FStar_Pervasives_Native.option ;
+  ls_source_root: source_root FStar_Pervasives_Native.option ;
+  ls_null_values: Prims.string Prims.list }
+let __proj__Mklogical_source__item__ls_iterator (projectee : logical_source)
+  : Prims.string FStar_Pervasives_Native.option=
+  match projectee with
+  | { ls_iterator; ls_reference_formulation; ls_source_path; ls_source_root;
+      ls_null_values;_} -> ls_iterator
+let __proj__Mklogical_source__item__ls_reference_formulation
+  (projectee : logical_source) :
+  reference_formulation FStar_Pervasives_Native.option=
+  match projectee with
+  | { ls_iterator; ls_reference_formulation; ls_source_path; ls_source_root;
+      ls_null_values;_} -> ls_reference_formulation
+let __proj__Mklogical_source__item__ls_source_path
+  (projectee : logical_source) : Prims.string FStar_Pervasives_Native.option=
+  match projectee with
+  | { ls_iterator; ls_reference_formulation; ls_source_path; ls_source_root;
+      ls_null_values;_} -> ls_source_path
+let __proj__Mklogical_source__item__ls_source_root
+  (projectee : logical_source) : source_root FStar_Pervasives_Native.option=
+  match projectee with
+  | { ls_iterator; ls_reference_formulation; ls_source_path; ls_source_root;
+      ls_null_values;_} -> ls_source_root
+let __proj__Mklogical_source__item__ls_null_values
+  (projectee : logical_source) : Prims.string Prims.list=
+  match projectee with
+  | { ls_iterator; ls_reference_formulation; ls_source_path; ls_source_root;
+      ls_null_values;_} -> ls_null_values
+let empty_logical_source : logical_source=
+  {
+    ls_iterator = FStar_Pervasives_Native.None;
+    ls_reference_formulation = FStar_Pervasives_Native.None;
+    ls_source_path = FStar_Pervasives_Native.None;
+    ls_source_root = FStar_Pervasives_Native.None;
+    ls_null_values = []
+  }
+let first_literal (l : RDF_Graph_Executable.rdf_term Prims.list) :
+  Prims.string FStar_Pervasives_Native.option=
+  match l with
+  | (RDF_Graph_Executable.T_Literal lit)::uu___ ->
+      FStar_Pervasives_Native.Some (lit.RDF_Graph_Executable.lexical_form)
+  | uu___ -> FStar_Pervasives_Native.None
+let literal_strings (l : RDF_Graph_Executable.rdf_term Prims.list) :
+  Prims.string Prims.list=
+  FStar_List_Tot_Base.concatMap
+    (fun t ->
+       match t with
+       | RDF_Graph_Executable.T_Literal lit ->
+           [lit.RDF_Graph_Executable.lexical_form]
+       | uu___ -> []) l
+let decode_logical_source (g : RDF_Graph_Executable.rdf_graph)
+  (s : RDF_Graph_Executable.subject) :
+  logical_source FStar_Pervasives_Native.option=
+  match RDF_Graph_Executable.find_objects g s rml_logicalSource with
+  | [] -> FStar_Pervasives_Native.None
+  | ls_term::uu___ ->
+      (match RDF_Graph_Executable.term_to_subject ls_term with
+       | FStar_Pervasives_Native.None -> FStar_Pervasives_Native.None
+       | FStar_Pervasives_Native.Some ls_subj ->
+           let iterator =
+             first_literal
+               (RDF_Graph_Executable.find_objects g ls_subj rml_iterator) in
+           let refform =
+             match RDF_Graph_Executable.find_objects g ls_subj
+                     rml_referenceFormulation
+             with
+             | t::uu___1 ->
+                 FStar_Pervasives_Native.Some
+                   (decode_reference_formulation t)
+             | [] -> FStar_Pervasives_Native.None in
+           let uu___1 =
+             match RDF_Graph_Executable.find_objects g ls_subj rml_source
+             with
+             | src_term::uu___2 ->
+                 (match RDF_Graph_Executable.term_to_subject src_term with
+                  | FStar_Pervasives_Native.Some src_subj ->
+                      ((first_literal
+                          (RDF_Graph_Executable.find_objects g src_subj
+                             rml_path)),
+                        ((match RDF_Graph_Executable.find_objects g src_subj
+                                  rml_root
+                          with
+                          | t::uu___3 ->
+                              FStar_Pervasives_Native.Some
+                                (decode_source_root t)
+                          | [] -> FStar_Pervasives_Native.None)),
+                        (literal_strings
+                           (RDF_Graph_Executable.find_objects g src_subj
+                              rml_null)))
+                  | FStar_Pervasives_Native.None ->
+                      (FStar_Pervasives_Native.None,
+                        FStar_Pervasives_Native.None, []))
+             | [] ->
+                 (FStar_Pervasives_Native.None, FStar_Pervasives_Native.None,
+                   []) in
+           (match uu___1 with
+            | (path, root, null_values) ->
+                FStar_Pervasives_Native.Some
+                  {
+                    ls_iterator = iterator;
+                    ls_reference_formulation = refform;
+                    ls_source_path = path;
+                    ls_source_root = root;
+                    ls_null_values = null_values
+                  }))
+type term_map_form =
+  | TMF_Constant of RDF_Graph_Executable.rdf_term 
+  | TMF_Reference of Prims.string 
+  | TMF_Template of Prims.string 
+  | TMF_Unknown 
+let uu___is_TMF_Constant (projectee : term_map_form) : Prims.bool=
+  match projectee with | TMF_Constant _0 -> true | uu___ -> false
+let __proj__TMF_Constant__item___0 (projectee : term_map_form) :
+  RDF_Graph_Executable.rdf_term= match projectee with | TMF_Constant _0 -> _0
+let uu___is_TMF_Reference (projectee : term_map_form) : Prims.bool=
+  match projectee with | TMF_Reference _0 -> true | uu___ -> false
+let __proj__TMF_Reference__item___0 (projectee : term_map_form) :
+  Prims.string= match projectee with | TMF_Reference _0 -> _0
+let uu___is_TMF_Template (projectee : term_map_form) : Prims.bool=
+  match projectee with | TMF_Template _0 -> true | uu___ -> false
+let __proj__TMF_Template__item___0 (projectee : term_map_form) :
+  Prims.string= match projectee with | TMF_Template _0 -> _0
+let uu___is_TMF_Unknown (projectee : term_map_form) : Prims.bool=
+  match projectee with | TMF_Unknown -> true | uu___ -> false
+type term_map =
+  {
+  tmap_form: term_map_form ;
+  tmap_termtype: term_type FStar_Pervasives_Native.option ;
+  tmap_datatype: term_map FStar_Pervasives_Native.option ;
+  tmap_language: term_map FStar_Pervasives_Native.option }
+let __proj__Mkterm_map__item__tmap_form (projectee : term_map) :
+  term_map_form=
+  match projectee with
+  | { tmap_form; tmap_termtype; tmap_datatype; tmap_language;_} -> tmap_form
+let __proj__Mkterm_map__item__tmap_termtype (projectee : term_map) :
+  term_type FStar_Pervasives_Native.option=
+  match projectee with
+  | { tmap_form; tmap_termtype; tmap_datatype; tmap_language;_} ->
+      tmap_termtype
+let __proj__Mkterm_map__item__tmap_datatype (projectee : term_map) :
+  term_map FStar_Pervasives_Native.option=
+  match projectee with
+  | { tmap_form; tmap_termtype; tmap_datatype; tmap_language;_} ->
+      tmap_datatype
+let __proj__Mkterm_map__item__tmap_language (projectee : term_map) :
+  term_map FStar_Pervasives_Native.option=
+  match projectee with
+  | { tmap_form; tmap_termtype; tmap_datatype; tmap_language;_} ->
+      tmap_language
+let unknown_term_map : term_map=
+  {
+    tmap_form = TMF_Unknown;
+    tmap_termtype = FStar_Pervasives_Native.None;
+    tmap_datatype = FStar_Pervasives_Native.None;
+    tmap_language = FStar_Pervasives_Native.None
+  }
+let const_term_map (t : RDF_Graph_Executable.rdf_term) : term_map=
+  {
+    tmap_form = (TMF_Constant t);
+    tmap_termtype = FStar_Pervasives_Native.None;
+    tmap_datatype = FStar_Pervasives_Native.None;
+    tmap_language = FStar_Pervasives_Native.None
+  }
+let ref_term_map (r : Prims.string) : term_map=
+  {
+    tmap_form = (TMF_Reference r);
+    tmap_termtype = FStar_Pervasives_Native.None;
+    tmap_datatype = FStar_Pervasives_Native.None;
+    tmap_language = FStar_Pervasives_Native.None
+  }
+let rec decode_term_map_from_subject (g : RDF_Graph_Executable.rdf_graph)
+  (s : RDF_Graph_Executable.subject) (fuel : Prims.nat) : term_map=
+  if fuel = Prims.int_zero
+  then unknown_term_map
+  else
+    (let fuel' = fuel - Prims.int_one in
+     let form =
+       match RDF_Graph_Executable.find_objects g s rml_constant with
+       | t::uu___1 -> TMF_Constant t
+       | [] ->
+           (match RDF_Graph_Executable.find_objects g s rml_reference with
+            | (RDF_Graph_Executable.T_Literal l)::uu___1 ->
+                TMF_Reference (l.RDF_Graph_Executable.lexical_form)
+            | uu___1 ->
+                (match RDF_Graph_Executable.find_objects g s rml_template
+                 with
+                 | (RDF_Graph_Executable.T_Literal l)::uu___2 ->
+                     TMF_Template (l.RDF_Graph_Executable.lexical_form)
+                 | uu___2 -> TMF_Unknown)) in
+     let termtype =
+       match RDF_Graph_Executable.find_objects g s rml_termType with
+       | t::uu___1 -> decode_term_type t
+       | [] -> FStar_Pervasives_Native.None in
+     let datatype =
+       match RDF_Graph_Executable.find_objects g s rml_datatypeMap with
+       | t::uu___1 ->
+           (match RDF_Graph_Executable.term_to_subject t with
+            | FStar_Pervasives_Native.Some ds ->
+                FStar_Pervasives_Native.Some
+                  (decode_term_map_from_subject g ds fuel')
+            | FStar_Pervasives_Native.None -> FStar_Pervasives_Native.None)
+       | [] ->
+           (match RDF_Graph_Executable.find_objects g s rml_datatype with
+            | t::uu___1 -> FStar_Pervasives_Native.Some (const_term_map t)
+            | [] -> FStar_Pervasives_Native.None) in
+     let language =
+       match RDF_Graph_Executable.find_objects g s rml_languageMap with
+       | t::uu___1 ->
+           (match RDF_Graph_Executable.term_to_subject t with
+            | FStar_Pervasives_Native.Some ls ->
+                FStar_Pervasives_Native.Some
+                  (decode_term_map_from_subject g ls fuel')
+            | FStar_Pervasives_Native.None -> FStar_Pervasives_Native.None)
+       | [] ->
+           (match RDF_Graph_Executable.find_objects g s rml_language with
+            | t::uu___1 -> FStar_Pervasives_Native.Some (const_term_map t)
+            | [] -> FStar_Pervasives_Native.None) in
+     {
+       tmap_form = form;
+       tmap_termtype = termtype;
+       tmap_datatype = datatype;
+       tmap_language = language
+     })
+type join_condition = {
+  jc_child: term_map ;
+  jc_parent: term_map }
+let __proj__Mkjoin_condition__item__jc_child (projectee : join_condition) :
+  term_map= match projectee with | { jc_child; jc_parent;_} -> jc_child
+let __proj__Mkjoin_condition__item__jc_parent (projectee : join_condition) :
+  term_map= match projectee with | { jc_child; jc_parent;_} -> jc_parent
+type ref_object_map =
+  {
+  rom_parent_triples_map: node_ref ;
+  rom_joins: join_condition Prims.list }
+let __proj__Mkref_object_map__item__rom_parent_triples_map
+  (projectee : ref_object_map) : node_ref=
+  match projectee with
+  | { rom_parent_triples_map; rom_joins;_} -> rom_parent_triples_map
+let __proj__Mkref_object_map__item__rom_joins (projectee : ref_object_map) :
+  join_condition Prims.list=
+  match projectee with | { rom_parent_triples_map; rom_joins;_} -> rom_joins
+let decode_child_or_parent (g : RDF_Graph_Executable.rdf_graph)
+  (s : RDF_Graph_Executable.subject) (map_pred : RDF_Graph_Executable.wf_iri)
+  (shortcut_pred : RDF_Graph_Executable.wf_iri) (fuel : Prims.nat) :
+  term_map=
+  match RDF_Graph_Executable.find_objects g s map_pred with
+  | t::uu___ ->
+      (match RDF_Graph_Executable.term_to_subject t with
+       | FStar_Pervasives_Native.Some ms ->
+           decode_term_map_from_subject g ms fuel
+       | FStar_Pervasives_Native.None -> unknown_term_map)
+  | [] ->
+      (match RDF_Graph_Executable.find_objects g s shortcut_pred with
+       | (RDF_Graph_Executable.T_Literal l)::uu___ ->
+           ref_term_map l.RDF_Graph_Executable.lexical_form
+       | uu___ -> unknown_term_map)
+let decode_join_conditions (g : RDF_Graph_Executable.rdf_graph)
+  (s : RDF_Graph_Executable.subject) (fuel : Prims.nat) :
+  join_condition Prims.list=
+  FStar_List_Tot_Base.concatMap
+    (fun t ->
+       match RDF_Graph_Executable.term_to_subject t with
+       | FStar_Pervasives_Native.None -> []
+       | FStar_Pervasives_Native.Some jc_subj ->
+           [{
+              jc_child =
+                (decode_child_or_parent g jc_subj rml_childMap rml_child fuel);
+              jc_parent =
+                (decode_child_or_parent g jc_subj rml_parentMap rml_parent
+                   fuel)
+            }]) (RDF_Graph_Executable.find_objects g s rml_joinCondition)
+type object_binding =
+  | OB_TermMap of term_map 
+  | OB_Join of ref_object_map 
+let uu___is_OB_TermMap (projectee : object_binding) : Prims.bool=
+  match projectee with | OB_TermMap _0 -> true | uu___ -> false
+let __proj__OB_TermMap__item___0 (projectee : object_binding) : term_map=
+  match projectee with | OB_TermMap _0 -> _0
+let uu___is_OB_Join (projectee : object_binding) : Prims.bool=
+  match projectee with | OB_Join _0 -> true | uu___ -> false
+let __proj__OB_Join__item___0 (projectee : object_binding) : ref_object_map=
+  match projectee with | OB_Join _0 -> _0
+type predicate_object_map =
+  {
+  pom_predicates: term_map Prims.list ;
+  pom_objects: object_binding Prims.list ;
+  pom_graphs: term_map Prims.list }
+let __proj__Mkpredicate_object_map__item__pom_predicates
+  (projectee : predicate_object_map) : term_map Prims.list=
+  match projectee with
+  | { pom_predicates; pom_objects; pom_graphs;_} -> pom_predicates
+let __proj__Mkpredicate_object_map__item__pom_objects
+  (projectee : predicate_object_map) : object_binding Prims.list=
+  match projectee with
+  | { pom_predicates; pom_objects; pom_graphs;_} -> pom_objects
+let __proj__Mkpredicate_object_map__item__pom_graphs
+  (projectee : predicate_object_map) : term_map Prims.list=
+  match projectee with
+  | { pom_predicates; pom_objects; pom_graphs;_} -> pom_graphs
+let decode_graphs (g : RDF_Graph_Executable.rdf_graph)
+  (s : RDF_Graph_Executable.subject) (fuel : Prims.nat) :
+  term_map Prims.list=
+  let via_map =
+    FStar_List_Tot_Base.concatMap
+      (fun t ->
+         match RDF_Graph_Executable.term_to_subject t with
+         | FStar_Pervasives_Native.Some gs ->
+             [decode_term_map_from_subject g gs fuel]
+         | FStar_Pervasives_Native.None -> [])
+      (RDF_Graph_Executable.find_objects g s rml_graphMap) in
+  let via_shortcut =
+    FStar_List_Tot_Base.map const_term_map
+      (RDF_Graph_Executable.find_objects g s rml_graph) in
+  FStar_List_Tot_Base.op_At via_map via_shortcut
+let decode_predicates (g : RDF_Graph_Executable.rdf_graph)
+  (s : RDF_Graph_Executable.subject) (fuel : Prims.nat) :
+  term_map Prims.list=
+  let via_map =
+    FStar_List_Tot_Base.concatMap
+      (fun t ->
+         match RDF_Graph_Executable.term_to_subject t with
+         | FStar_Pervasives_Native.Some ps ->
+             [decode_term_map_from_subject g ps fuel]
+         | FStar_Pervasives_Native.None -> [])
+      (RDF_Graph_Executable.find_objects g s rml_predicateMap) in
+  let via_shortcut =
+    FStar_List_Tot_Base.map const_term_map
+      (RDF_Graph_Executable.find_objects g s rml_predicate) in
+  FStar_List_Tot_Base.op_At via_map via_shortcut
+let decode_object_bindings (g : RDF_Graph_Executable.rdf_graph)
+  (s : RDF_Graph_Executable.subject) (fuel : Prims.nat) :
+  object_binding Prims.list=
+  let via_object_map =
+    FStar_List_Tot_Base.concatMap
+      (fun t ->
+         match RDF_Graph_Executable.term_to_subject t with
+         | FStar_Pervasives_Native.None -> []
+         | FStar_Pervasives_Native.Some om_subj ->
+             (match RDF_Graph_Executable.find_objects g om_subj
+                      rml_parentTriplesMap
+              with
+              | ptm::uu___ ->
+                  let parent_ref =
+                    match term_to_node_ref ptm with
+                    | FStar_Pervasives_Native.Some r -> r
+                    | FStar_Pervasives_Native.None -> "" in
+                  [OB_Join
+                     {
+                       rom_parent_triples_map = parent_ref;
+                       rom_joins = (decode_join_conditions g om_subj fuel)
+                     }]
+              | [] ->
+                  [OB_TermMap (decode_term_map_from_subject g om_subj fuel)]))
+      (RDF_Graph_Executable.find_objects g s rml_objectMap) in
+  let via_object_shortcut =
+    FStar_List_Tot_Base.map (fun t -> OB_TermMap (const_term_map t))
+      (RDF_Graph_Executable.find_objects g s rml_object) in
+  FStar_List_Tot_Base.op_At via_object_map via_object_shortcut
+let decode_predicate_object_map (g : RDF_Graph_Executable.rdf_graph)
+  (pom_subj : RDF_Graph_Executable.subject) (fuel : Prims.nat) :
+  predicate_object_map=
+  {
+    pom_predicates = (decode_predicates g pom_subj fuel);
+    pom_objects = (decode_object_bindings g pom_subj fuel);
+    pom_graphs = (decode_graphs g pom_subj fuel)
+  }
+let decode_predicate_object_maps (g : RDF_Graph_Executable.rdf_graph)
+  (s : RDF_Graph_Executable.subject) (fuel : Prims.nat) :
+  predicate_object_map Prims.list=
+  FStar_List_Tot_Base.concatMap
+    (fun t ->
+       match RDF_Graph_Executable.term_to_subject t with
+       | FStar_Pervasives_Native.Some pom_subj ->
+           [decode_predicate_object_map g pom_subj fuel]
+       | FStar_Pervasives_Native.None -> [])
+    (RDF_Graph_Executable.find_objects g s rml_predicateObjectMap)
+type subject_map_t =
+  {
+  sm_term: term_map ;
+  sm_classes: RDF_Graph_Executable.wf_iri Prims.list ;
+  sm_graphs: term_map Prims.list }
+let __proj__Mksubject_map_t__item__sm_term (projectee : subject_map_t) :
+  term_map=
+  match projectee with | { sm_term; sm_classes; sm_graphs;_} -> sm_term
+let __proj__Mksubject_map_t__item__sm_classes (projectee : subject_map_t) :
+  RDF_Graph_Executable.wf_iri Prims.list=
+  match projectee with | { sm_term; sm_classes; sm_graphs;_} -> sm_classes
+let __proj__Mksubject_map_t__item__sm_graphs (projectee : subject_map_t) :
+  term_map Prims.list=
+  match projectee with | { sm_term; sm_classes; sm_graphs;_} -> sm_graphs
+let decode_subject_map (g : RDF_Graph_Executable.rdf_graph)
+  (s : RDF_Graph_Executable.subject) (fuel : Prims.nat) :
+  subject_map_t FStar_Pervasives_Native.option=
+  match RDF_Graph_Executable.find_objects g s rml_subjectMap with
+  | [] ->
+      (match RDF_Graph_Executable.find_objects g s rml_subject with
+       | t::uu___ ->
+           FStar_Pervasives_Native.Some
+             { sm_term = (const_term_map t); sm_classes = []; sm_graphs = []
+             }
+       | [] -> FStar_Pervasives_Native.None)
+  | sm_term::[] ->
+      (match RDF_Graph_Executable.term_to_subject sm_term with
+       | FStar_Pervasives_Native.None -> FStar_Pervasives_Native.None
+       | FStar_Pervasives_Native.Some sm_subj ->
+           let term = decode_term_map_from_subject g sm_subj fuel in
+           let classes =
+             FStar_List_Tot_Base.concatMap
+               (fun t ->
+                  match t with
+                  | RDF_Graph_Executable.T_IRI i -> [i]
+                  | uu___ -> [])
+               (RDF_Graph_Executable.find_objects g sm_subj rml_class) in
+           let graphs = decode_graphs g sm_subj fuel in
+           FStar_Pervasives_Native.Some
+             { sm_term = term; sm_classes = classes; sm_graphs = graphs })
+  | uu___::uu___1::uu___2 -> FStar_Pervasives_Native.None
+type triples_map =
+  {
+  tm_id: node_ref ;
+  tm_base_iri: Prims.string FStar_Pervasives_Native.option ;
+  tm_logical_source: logical_source FStar_Pervasives_Native.option ;
+  tm_subject_map: subject_map_t FStar_Pervasives_Native.option ;
+  tm_predicate_object_maps: predicate_object_map Prims.list }
+let __proj__Mktriples_map__item__tm_id (projectee : triples_map) : node_ref=
+  match projectee with
+  | { tm_id; tm_base_iri; tm_logical_source; tm_subject_map;
+      tm_predicate_object_maps;_} -> tm_id
+let __proj__Mktriples_map__item__tm_base_iri (projectee : triples_map) :
+  Prims.string FStar_Pervasives_Native.option=
+  match projectee with
+  | { tm_id; tm_base_iri; tm_logical_source; tm_subject_map;
+      tm_predicate_object_maps;_} -> tm_base_iri
+let __proj__Mktriples_map__item__tm_logical_source (projectee : triples_map)
+  : logical_source FStar_Pervasives_Native.option=
+  match projectee with
+  | { tm_id; tm_base_iri; tm_logical_source; tm_subject_map;
+      tm_predicate_object_maps;_} -> tm_logical_source
+let __proj__Mktriples_map__item__tm_subject_map (projectee : triples_map) :
+  subject_map_t FStar_Pervasives_Native.option=
+  match projectee with
+  | { tm_id; tm_base_iri; tm_logical_source; tm_subject_map;
+      tm_predicate_object_maps;_} -> tm_subject_map
+let __proj__Mktriples_map__item__tm_predicate_object_maps
+  (projectee : triples_map) : predicate_object_map Prims.list=
+  match projectee with
+  | { tm_id; tm_base_iri; tm_logical_source; tm_subject_map;
+      tm_predicate_object_maps;_} -> tm_predicate_object_maps
+type mapping_document = {
+  md_triples_maps: triples_map Prims.list }
+let __proj__Mkmapping_document__item__md_triples_maps
+  (projectee : mapping_document) : triples_map Prims.list=
+  match projectee with | { md_triples_maps;_} -> md_triples_maps
+let decode_triples_map (g : RDF_Graph_Executable.rdf_graph)
+  (s : RDF_Graph_Executable.subject) (fuel : Prims.nat) : triples_map=
+  {
+    tm_id = (subject_to_node_ref s);
+    tm_base_iri =
+      (match RDF_Graph_Executable.find_objects g s rml_baseIRI with
+       | (RDF_Graph_Executable.T_IRI i)::uu___ ->
+           FStar_Pervasives_Native.Some i
+       | uu___ -> FStar_Pervasives_Native.None);
+    tm_logical_source = (decode_logical_source g s);
+    tm_subject_map = (decode_subject_map g s fuel);
+    tm_predicate_object_maps = (decode_predicate_object_maps g s fuel)
+  }
+let is_triples_map_subject (g : RDF_Graph_Executable.rdf_graph)
+  (s : RDF_Graph_Executable.subject) : Prims.bool=
+  FStar_List_Tot_Base.existsb
+    (fun t ->
+       ((RDF_Graph_Executable.subject_eq t.RDF_Graph_Executable.s s) &&
+          (t.RDF_Graph_Executable.p = RDF_Graph_Executable.rdf_type))
+         &&
+         (RDF_Graph_Executable.rdf_term_eq t.RDF_Graph_Executable.o
+            (RDF_Graph_Executable.T_IRI rml_TriplesMap))) g
+let decode_mapping_document (g : RDF_Graph_Executable.rdf_graph) :
+  mapping_document=
+  let subs = distinct_subjects g in
+  let tm_subs = FStar_List_Tot_Base.filter (is_triples_map_subject g) subs in
+  {
+    md_triples_maps =
+      (FStar_List_Tot_Base.map
+         (fun s ->
+            decode_triples_map g s
+              ((RDF_Graph_Executable.graph_len g) + Prims.int_one)) tm_subs)
+  }
